Regex/Syntax/Hir.lean
@@ -1,53 +1,7 @@
 import Regex.Regex
-import Regex.Intervals
+import Regex.Classes
 
 namespace Regex.Syntax.Parser
-
-inductive PerlClassKind where
-  | digit
-  | space
-  | word
-deriving Repr
-
--- NOTE: we may want to interpret these as Unicode character properties in the future
-def PerlClassKind.toRange : PerlClassKind → Intervals
-  | .digit => #[⟨('0', '9'), by decide⟩]
-  | .space => #[⟨(' ', ' '), by decide⟩, ⟨('\t', '\t'), by decide⟩, ⟨('\n', '\n'), by decide⟩, ⟨('\r', '\r'), by decide⟩, ⟨('\x0B', '\x0B'), by decide⟩, ⟨('\x0C', '\x0C'), by decide⟩]
-  | .word => #[⟨('a', 'z'), by decide⟩, ⟨('A', 'Z'), by decide⟩, ⟨('0', '9'), by decide⟩, ⟨('_', '_'), by decide⟩]
-
-structure PerlClass where
-  negated : Bool
-  kind : PerlClassKind
-deriving Repr
-
-def PerlClass.toRange (perl: PerlClass) : Intervals :=
-  if perl.negated
-    then Intervals.invert perl.kind.toRange
-    else perl.kind.toRange
-
--- NOTE: s ≤ e prevents this from deriving Repr :(
-inductive Interval where
-  | single : Char → Interval
-  | range : (s : Char) → (e : Char) → s ≤ e → Interval
-  | perl : PerlClass → Interval
-
-def Interval.toRange : Interval → Intervals
-  | .single c      => #[⟨(c, c), by simp⟩]
-  | .range c₁ c₂ r => #[⟨(c₁, c₂), r⟩]
-  | .perl p        => p.toRange
-
-structure Classes where
-  negated : Bool
-  intervals : Array Interval
-
-def Classes.toRange (classes: Classes) : Intervals :=
-  let intervals := Array.concatMap (·.toRange) classes.intervals
-
-  let intervals₁ : Intervals := if classes.negated
-    then Intervals.invert intervals
-    else intervals
-
-  Intervals.merge intervals₁
 
 inductive Hir : Type where
   | empty : Hir
@@ -81,11 +35,9 @@ def Hir.toRegexAux (index : Nat) (hir : Hir) : Nat × Regex :=
   | .star h =>
     let (index', r) := h.toRegexAux index
     (index', .star r)
-  | .classes c =>
-    (index, .classes c.toRange)
-  | .perl p =>
-    (index, .classes p.toRange)
-  | .dot => (index, .classes #[⟨(Char.ofNat 0, Char.ofNat Char.MAX_UNICODE), by decide⟩])
+  | .classes cs => (index, .classes cs)
+  | .perl pc => (index, .classes ⟨false, #[Class.perl pc]⟩)
+  | .dot => (index, .classes ⟨false, #[Class.any]⟩)
 
 def Hir.toRegex (h : Hir) : Regex := (h.toRegexAux 0).2
 
